securedrop-protocol/protocol-minimal/proofs/fstar/extraction/Securedrop_protocol_minimal.Journalist.fst
@@ -1,0 +1,30 @@
+module Securedrop_protocol_minimal.Journalist
+#set-options "--fuel 0 --ifuel 1 --z3rlimit 15"
+open FStar.Mul
+open Core_models
+
+include Securedrop_protocol_minimal.Bundle {impl__from__journalist as impl}
+
+include Securedrop_protocol_minimal.Bundle {impl_1__from__journalist as impl_1}
+
+include Securedrop_protocol_minimal.Bundle {t_Journalist as t_Journalist}
+
+include Securedrop_protocol_minimal.Bundle {t_JournalistPublicView as t_JournalistPublicView}
+
+include Securedrop_protocol_minimal.Bundle {impl_2__new as impl_JournalistPublicView__new}
+
+include Securedrop_protocol_minimal.Bundle {impl_3 as impl_3}
+
+include Securedrop_protocol_minimal.Bundle {impl_4 as impl_4}
+
+include Securedrop_protocol_minimal.Bundle {impl_5 as impl_5}
+
+include Securedrop_protocol_minimal.Bundle {impl_6 as impl_6}
+
+include Securedrop_protocol_minimal.Bundle {impl_7 as impl_7}
+
+include Securedrop_protocol_minimal.Bundle {f_signed_keybundles__impl_7__extract_public_bundle as f_signed_keybundles__impl_7__extract_public_bundle}
+
+include Securedrop_protocol_minimal.Bundle {impl_8__new as impl_Journalist__new}
+
+include Securedrop_protocol_minimal.Bundle {impl_8__public as impl_Journalist__public}
