securedrop-protocol/protocol-minimal/proofs/fstar/extraction/Securedrop_protocol_minimal.Sign.fst
@@ -1,0 +1,542 @@
+module Securedrop_protocol_minimal.Sign
+#set-options "--fuel 0 --ifuel 1 --z3rlimit 15"
+open FStar.Mul
+open Core_models
+
+let _ =
+  (* This module has implicit dependencies, here we make them explicit. *)
+  (* The implicit dependencies arise from typeclasses instances. *)
+  let open Libcrux_ed25519.Impl_hacl in
+  let open Rand_core in
+  let open Securedrop_protocol_minimal.Sign.Private in
+  ()
+
+/// Marker trait for signature domain separation.
+/// Each impl encodes the ASCII tag that is prepended to every signing preimage
+/// in that domain: `len(tag) || tag || msg`  (see footnote in the spec).
+class t_DomainTag (v_Self: Type0) = {
+  [@@@ FStar.Tactics.Typeclasses.no_method]_super_i0:Securedrop_protocol_minimal.Sign.Private.t_Sealed
+  v_Self;
+  f_TAG:t_Slice u8
+}
+
+[@@ FStar.Tactics.Typeclasses.tcinstance]
+let _ = fun (v_Self:Type0) {|i: t_DomainTag v_Self|} -> i._super_i0
+
+/// Journalist self-signature over long-term public keys (step 3.1).
+type t_JournalistLongTermKey = | JournalistLongTermKey : t_JournalistLongTermKey
+
+[@@ FStar.Tactics.Typeclasses.tcinstance]
+assume
+val impl_15': Core_models.Fmt.t_Debug t_JournalistLongTermKey
+
+unfold
+let impl_15 = impl_15'
+
+let impl_16: Core_models.Clone.t_Clone t_JournalistLongTermKey =
+  { f_clone = (fun x -> x); f_clone_pre = (fun _ -> True); f_clone_post = (fun _ _ -> True) }
+
+[@@ FStar.Tactics.Typeclasses.tcinstance]
+assume
+val impl_17': Core_models.Marker.t_Copy t_JournalistLongTermKey
+
+unfold
+let impl_17 = impl_17'
+
+[@@ FStar.Tactics.Typeclasses.tcinstance]
+assume
+val impl_18': Core_models.Marker.t_StructuralPartialEq t_JournalistLongTermKey
+
+unfold
+let impl_18 = impl_18'
+
+[@@ FStar.Tactics.Typeclasses.tcinstance]
+assume
+val impl_19': Core_models.Cmp.t_PartialEq t_JournalistLongTermKey t_JournalistLongTermKey
+
+unfold
+let impl_19 = impl_19'
+
+[@@ FStar.Tactics.Typeclasses.tcinstance]
+assume
+val impl_20': Core_models.Cmp.t_Eq t_JournalistLongTermKey
+
+unfold
+let impl_20 = impl_20'
+
+/// Journalist self-signature over ephemeral key bundles (step 3.2).
+type t_JournalistEphemeralKey = | JournalistEphemeralKey : t_JournalistEphemeralKey
+
+[@@ FStar.Tactics.Typeclasses.tcinstance]
+assume
+val impl_21': Core_models.Fmt.t_Debug t_JournalistEphemeralKey
+
+unfold
+let impl_21 = impl_21'
+
+let impl_22: Core_models.Clone.t_Clone t_JournalistEphemeralKey =
+  { f_clone = (fun x -> x); f_clone_pre = (fun _ -> True); f_clone_post = (fun _ _ -> True) }
+
+[@@ FStar.Tactics.Typeclasses.tcinstance]
+assume
+val impl_23': Core_models.Marker.t_Copy t_JournalistEphemeralKey
+
+unfold
+let impl_23 = impl_23'
+
+[@@ FStar.Tactics.Typeclasses.tcinstance]
+assume
+val impl_24': Core_models.Marker.t_StructuralPartialEq t_JournalistEphemeralKey
+
+unfold
+let impl_24 = impl_24'
+
+[@@ FStar.Tactics.Typeclasses.tcinstance]
+assume
+val impl_25': Core_models.Cmp.t_PartialEq t_JournalistEphemeralKey t_JournalistEphemeralKey
+
+unfold
+let impl_25 = impl_25'
+
+[@@ FStar.Tactics.Typeclasses.tcinstance]
+assume
+val impl_26': Core_models.Cmp.t_Eq t_JournalistEphemeralKey
+
+unfold
+let impl_26 = impl_26'
+
+/// Newsroom signature over a journalist's verifying key (steps 3.1, 5).
+type t_NewsroomOnJournalist = | NewsroomOnJournalist : t_NewsroomOnJournalist
+
+[@@ FStar.Tactics.Typeclasses.tcinstance]
+assume
+val impl_27': Core_models.Fmt.t_Debug t_NewsroomOnJournalist
+
+unfold
+let impl_27 = impl_27'
+
+let impl_28: Core_models.Clone.t_Clone t_NewsroomOnJournalist =
+  { f_clone = (fun x -> x); f_clone_pre = (fun _ -> True); f_clone_post = (fun _ _ -> True) }
+
+[@@ FStar.Tactics.Typeclasses.tcinstance]
+assume
+val impl_29': Core_models.Marker.t_Copy t_NewsroomOnJournalist
+
+unfold
+let impl_29 = impl_29'
+
+[@@ FStar.Tactics.Typeclasses.tcinstance]
+assume
+val impl_30': Core_models.Marker.t_StructuralPartialEq t_NewsroomOnJournalist
+
+unfold
+let impl_30 = impl_30'
+
+[@@ FStar.Tactics.Typeclasses.tcinstance]
+assume
+val impl_31': Core_models.Cmp.t_PartialEq t_NewsroomOnJournalist t_NewsroomOnJournalist
+
+unfold
+let impl_31 = impl_31'
+
+[@@ FStar.Tactics.Typeclasses.tcinstance]
+assume
+val impl_32': Core_models.Cmp.t_Eq t_NewsroomOnJournalist
+
+unfold
+let impl_32 = impl_32'
+
+/// FPF signature over the newsroom's verifying key (step 2).
+type t_FpfOnNewsroom = | FpfOnNewsroom : t_FpfOnNewsroom
+
+[@@ FStar.Tactics.Typeclasses.tcinstance]
+assume
+val impl_33': Core_models.Fmt.t_Debug t_FpfOnNewsroom
+
+unfold
+let impl_33 = impl_33'
+
+let impl_34: Core_models.Clone.t_Clone t_FpfOnNewsroom =
+  { f_clone = (fun x -> x); f_clone_pre = (fun _ -> True); f_clone_post = (fun _ _ -> True) }
+
+[@@ FStar.Tactics.Typeclasses.tcinstance]
+assume
+val impl_35': Core_models.Marker.t_Copy t_FpfOnNewsroom
+
+unfold
+let impl_35 = impl_35'
+
+[@@ FStar.Tactics.Typeclasses.tcinstance]
+assume
+val impl_36': Core_models.Marker.t_StructuralPartialEq t_FpfOnNewsroom
+
+unfold
+let impl_36 = impl_36'
+
+[@@ FStar.Tactics.Typeclasses.tcinstance]
+assume
+val impl_37': Core_models.Cmp.t_PartialEq t_FpfOnNewsroom t_FpfOnNewsroom
+
+unfold
+let impl_37 = impl_37'
+
+[@@ FStar.Tactics.Typeclasses.tcinstance]
+assume
+val impl_38': Core_models.Cmp.t_Eq t_FpfOnNewsroom
+
+unfold
+let impl_38 = impl_38'
+
+[@@ FStar.Tactics.Typeclasses.tcinstance]
+let impl: Securedrop_protocol_minimal.Sign.Private.t_Sealed t_JournalistLongTermKey =
+  { __marker_trait_Securedrop_protocol_minimal.Sign.Private.t_Sealed = () }
+
+[@@ FStar.Tactics.Typeclasses.tcinstance]
+let impl_1: Securedrop_protocol_minimal.Sign.Private.t_Sealed t_JournalistEphemeralKey =
+  { __marker_trait_Securedrop_protocol_minimal.Sign.Private.t_Sealed = () }
+
+[@@ FStar.Tactics.Typeclasses.tcinstance]
+let impl_2: Securedrop_protocol_minimal.Sign.Private.t_Sealed t_NewsroomOnJournalist =
+  { __marker_trait_Securedrop_protocol_minimal.Sign.Private.t_Sealed = () }
+
+[@@ FStar.Tactics.Typeclasses.tcinstance]
+let impl_3: Securedrop_protocol_minimal.Sign.Private.t_Sealed t_FpfOnNewsroom =
+  { __marker_trait_Securedrop_protocol_minimal.Sign.Private.t_Sealed = () }
+
+[@@ FStar.Tactics.Typeclasses.tcinstance]
+let impl_DomainTag_for_JournalistLongTermKey: t_DomainTag t_JournalistLongTermKey =
+  {
+    _super_i0 = FStar.Tactics.Typeclasses.solve;
+    f_TAG
+    =
+    (let list =
+        [
+          mk_u8 106;
+          mk_u8 45;
+          mk_u8 115;
+          mk_u8 105;
+          mk_u8 103;
+          mk_u8 45;
+          mk_u8 108;
+          mk_u8 116;
+          mk_u8 107
+        ]
+      in
+      FStar.Pervasives.assert_norm (Prims.eq2 (List.Tot.length list) 9);
+      Rust_primitives.Hax.array_of_list 9 list)
+    <:
+    t_Slice u8
+  }
+
+[@@ FStar.Tactics.Typeclasses.tcinstance]
+let impl_DomainTag_for_JournalistEphemeralKey: t_DomainTag t_JournalistEphemeralKey =
+  {
+    _super_i0 = FStar.Tactics.Typeclasses.solve;
+    f_TAG
+    =
+    (let list =
+        [
+          mk_u8 106;
+          mk_u8 45;
+          mk_u8 115;
+          mk_u8 105;
+          mk_u8 103;
+          mk_u8 45;
+          mk_u8 101;
+          mk_u8 112;
+          mk_u8 104
+        ]
+      in
+      FStar.Pervasives.assert_norm (Prims.eq2 (List.Tot.length list) 9);
+      Rust_primitives.Hax.array_of_list 9 list)
+    <:
+    t_Slice u8
+  }
+
+[@@ FStar.Tactics.Typeclasses.tcinstance]
+let impl_DomainTag_for_NewsroomOnJournalist: t_DomainTag t_NewsroomOnJournalist =
+  {
+    _super_i0 = FStar.Tactics.Typeclasses.solve;
+    f_TAG
+    =
+    (let list = [mk_u8 110; mk_u8 114; mk_u8 45; mk_u8 115; mk_u8 105; mk_u8 103] in
+      FStar.Pervasives.assert_norm (Prims.eq2 (List.Tot.length list) 6);
+      Rust_primitives.Hax.array_of_list 6 list)
+    <:
+    t_Slice u8
+  }
+
+[@@ FStar.Tactics.Typeclasses.tcinstance]
+let impl_DomainTag_for_FpfOnNewsroom: t_DomainTag t_FpfOnNewsroom =
+  {
+    _super_i0 = FStar.Tactics.Typeclasses.solve;
+    f_TAG
+    =
+    (let list =
+        [
+          mk_u8 102; mk_u8 112; mk_u8 102; mk_u8 45; mk_u8 115; mk_u8 105; mk_u8 103; mk_u8 45;
+          mk_u8 110; mk_u8 114
+        ]
+      in
+      FStar.Pervasives.assert_norm (Prims.eq2 (List.Tot.length list) 10);
+      Rust_primitives.Hax.array_of_list 10 list)
+    <:
+    t_Slice u8
+  }
+
+/// An Ed25519 signature carrying its domain at the type level.
+/// A `Signature<D>` can only be verified against a message using the same
+/// domain `D`, making cross-domain misuse a compile error rather than a
+/// runtime failure.
+type t_Signature (v_D: Type0) {| i0: t_DomainTag v_D |} = {
+  f_bytes:t_Array u8 (mk_usize 64);
+  f_e_phantom:Core_models.Marker.t_PhantomData (Prims.unit -> v_D)
+}
+
+[@@ FStar.Tactics.Typeclasses.tcinstance]
+let impl_9 (#v_D: Type0) (#[FStar.Tactics.Typeclasses.tcresolve ()] i0: t_DomainTag v_D)
+    : Core_models.Clone.t_Clone (t_Signature v_D) =
+  {
+    f_clone_pre = (fun (self: t_Signature v_D) -> true);
+    f_clone_post = (fun (self: t_Signature v_D) (out: t_Signature v_D) -> true);
+    f_clone = fun (self: t_Signature v_D) -> self
+  }
+
+[@@ FStar.Tactics.Typeclasses.tcinstance]
+let impl_8 (#v_D: Type0) (#[FStar.Tactics.Typeclasses.tcresolve ()] i0: t_DomainTag v_D)
+    : Core_models.Marker.t_Copy (t_Signature v_D) = { _super_i0 = FStar.Tactics.Typeclasses.solve }
+
+[@@ FStar.Tactics.Typeclasses.tcinstance]
+let impl_10 (#v_D: Type0) (#[FStar.Tactics.Typeclasses.tcresolve ()] i0: t_DomainTag v_D)
+    : Core_models.Cmp.t_PartialEq (t_Signature v_D) (t_Signature v_D) =
+  {
+    f_eq_pre = (fun (self: t_Signature v_D) (other: t_Signature v_D) -> true);
+    f_eq_post = (fun (self: t_Signature v_D) (other: t_Signature v_D) (out: bool) -> true);
+    f_eq = fun (self: t_Signature v_D) (other: t_Signature v_D) -> self.f_bytes =. other.f_bytes
+  }
+
+[@@ FStar.Tactics.Typeclasses.tcinstance]
+let impl_11 (#v_D: Type0) (#[FStar.Tactics.Typeclasses.tcresolve ()] i0: t_DomainTag v_D)
+    : Core_models.Cmp.t_Eq (t_Signature v_D) = { _super_i0 = FStar.Tactics.Typeclasses.solve }
+
+let impl_12__from_bytes
+      (#v_D: Type0)
+      (#[FStar.Tactics.Typeclasses.tcresolve ()] i0: t_DomainTag v_D)
+      (bytes: t_Array u8 (mk_usize 64))
+    : t_Signature v_D =
+  {
+    f_bytes = bytes;
+    f_e_phantom
+    =
+    Core_models.Marker.PhantomData <: Core_models.Marker.t_PhantomData (Prims.unit -> v_D)
+  }
+  <:
+  t_Signature v_D
+
+/// Construct the tagged signing preimage: `len(tag) || tag || msg`.
+let tagged_preimage
+      (#v_D: Type0)
+      (#[FStar.Tactics.Typeclasses.tcresolve ()] i0: t_DomainTag v_D)
+      (msg: t_Slice u8)
+    : Alloc.Vec.t_Vec u8 Alloc.Alloc.t_Global =
+  let tag:t_Slice u8 = f_TAG #FStar.Tactics.Typeclasses.solve in
+  let _:Prims.unit =
+    if true
+    then
+      let _:Prims.unit =
+        if ~.((Core_models.Slice.impl__len #u8 tag <: usize) <=. mk_usize 255 <: bool)
+        then
+          Rust_primitives.Hax.never_to_any (Core_models.Panicking.panic_fmt (Core_models.Fmt.Rt.impl_1__new_const
+                    (mk_usize 1)
+                    (let list = ["tag length exceeds u8::MAX"] in
+                      FStar.Pervasives.assert_norm (Prims.eq2 (List.Tot.length list) 1);
+                      Rust_primitives.Hax.array_of_list 1 list)
+                  <:
+                  Core_models.Fmt.t_Arguments)
+              <:
+              Rust_primitives.Hax.t_Never)
+      in
+      ()
+  in
+  let _:Prims.unit =
+    if true
+    then
+      let _:Prims.unit =
+        if ~.(Core_models.Slice.Ascii.impl_slice_of_u8__is_ascii tag <: bool)
+        then
+          Rust_primitives.Hax.never_to_any (Core_models.Panicking.panic_fmt (Core_models.Fmt.Rt.impl_1__new_const
+                    (mk_usize 1)
+                    (let list = ["tag contains non-ASCII bytes"] in
+                      FStar.Pervasives.assert_norm (Prims.eq2 (List.Tot.length list) 1);
+                      Rust_primitives.Hax.array_of_list 1 list)
+                  <:
+                  Core_models.Fmt.t_Arguments)
+              <:
+              Rust_primitives.Hax.t_Never)
+      in
+      ()
+  in
+  let preimage:Alloc.Vec.t_Vec u8 Alloc.Alloc.t_Global =
+    Alloc.Vec.impl__with_capacity #u8
+      ((mk_usize 1 +! (Core_models.Slice.impl__len #u8 tag <: usize) <: usize) +!
+        (Core_models.Slice.impl__len #u8 msg <: usize)
+        <:
+        usize)
+  in
+  let preimage:Alloc.Vec.t_Vec u8 Alloc.Alloc.t_Global =
+    Alloc.Vec.impl_1__push #u8
+      #Alloc.Alloc.t_Global
+      preimage
+      (cast (Core_models.Slice.impl__len #u8 tag <: usize) <: u8)
+  in
+  let preimage:Alloc.Vec.t_Vec u8 Alloc.Alloc.t_Global =
+    Alloc.Vec.impl_2__extend_from_slice #u8 #Alloc.Alloc.t_Global preimage tag
+  in
+  let preimage:Alloc.Vec.t_Vec u8 Alloc.Alloc.t_Global =
+    Alloc.Vec.impl_2__extend_from_slice #u8 #Alloc.Alloc.t_Global preimage msg
+  in
+  preimage
+
+/// An Ed25519 verification key.
+type t_VerifyingKey = | VerifyingKey : Libcrux_ed25519.Impl_hacl.t_VerificationKey -> t_VerifyingKey
+
+/// An Ed25519 signing key.
+type t_SigningKey = {
+  f_vk:t_VerifyingKey;
+  f_sk:Libcrux_ed25519.Impl_hacl.t_SigningKey
+}
+
+let impl_42: Core_models.Clone.t_Clone t_VerifyingKey =
+  { f_clone = (fun x -> x); f_clone_pre = (fun _ -> True); f_clone_post = (fun _ _ -> True) }
+
+[@@ FStar.Tactics.Typeclasses.tcinstance]
+assume
+val impl_41': Core_models.Marker.t_Copy t_VerifyingKey
+
+unfold
+let impl_41 = impl_41'
+
+/// Generate a signing key from the supplied `rng`.
+let impl_SigningKey__new
+      (#v_R: Type0)
+      (#[FStar.Tactics.Typeclasses.tcresolve ()] i0: Rand_core.t_CryptoRng v_R)
+      (rng: v_R)
+    : (v_R & Core_models.Result.t_Result t_SigningKey Anyhow.t_Error) =
+  let
+  (tmp0: v_R),
+  (out:
+    Core_models.Result.t_Result
+      (Libcrux_ed25519.Impl_hacl.t_SigningKey & Libcrux_ed25519.Impl_hacl.t_VerificationKey)
+      Libcrux_ed25519.Impl_hacl.t_Error) =
+    Libcrux_ed25519.Impl_hacl.generate_key_pair #v_R rng
+  in
+  let rng:v_R = tmp0 in
+  match
+    Core_models.Result.impl__map_err #(Libcrux_ed25519.Impl_hacl.t_SigningKey &
+        Libcrux_ed25519.Impl_hacl.t_VerificationKey)
+      #Libcrux_ed25519.Impl_hacl.t_Error
+      #Anyhow.t_Error
+      out
+      (fun temp_0_ ->
+          let _:Libcrux_ed25519.Impl_hacl.t_Error = temp_0_ in
+          let error:Anyhow.t_Error =
+            Anyhow.__private.format_err (Core_models.Fmt.Rt.impl_1__new_const (mk_usize 1)
+                  (let list = ["Key generation failed"] in
+                    FStar.Pervasives.assert_norm (Prims.eq2 (List.Tot.length list) 1);
+                    Rust_primitives.Hax.array_of_list 1 list)
+                <:
+                Core_models.Fmt.t_Arguments)
+          in
+          Anyhow.__private.must_use error)
+    <:
+    Core_models.Result.t_Result
+      (Libcrux_ed25519.Impl_hacl.t_SigningKey & Libcrux_ed25519.Impl_hacl.t_VerificationKey)
+      Anyhow.t_Error
+  with
+  | Core_models.Result.Result_Ok (sk, vk) ->
+    let hax_temp_output:Core_models.Result.t_Result t_SigningKey Anyhow.t_Error =
+      Core_models.Result.Result_Ok
+      ({ f_vk = VerifyingKey vk <: t_VerifyingKey; f_sk = sk } <: t_SigningKey)
+      <:
+      Core_models.Result.t_Result t_SigningKey Anyhow.t_Error
+    in
+    rng, hax_temp_output <: (v_R & Core_models.Result.t_Result t_SigningKey Anyhow.t_Error)
+  | Core_models.Result.Result_Err err ->
+    rng,
+    (Core_models.Result.Result_Err err <: Core_models.Result.t_Result t_SigningKey Anyhow.t_Error)
+    <:
+    (v_R & Core_models.Result.t_Result t_SigningKey Anyhow.t_Error)
+
+/// Sign `msg` in domain `D`, returning a `Signature<D>`.
+/// The actual preimage is `len(tag) || tag || msg` where `tag = D::TAG`.
+let impl_SigningKey__sign
+      (#v_D: Type0)
+      (#[FStar.Tactics.Typeclasses.tcresolve ()] i0: t_DomainTag v_D)
+      (self: t_SigningKey)
+      (msg: t_Slice u8)
+    : t_Signature v_D =
+  let preimage:Alloc.Vec.t_Vec u8 Alloc.Alloc.t_Global = tagged_preimage #v_D msg in
+  let bytes:t_Array u8 (mk_usize 64) =
+    Core_models.Result.impl__expect #(t_Array u8 (mk_usize 64))
+      #Libcrux_ed25519.Impl_hacl.t_Error
+      (Libcrux_ed25519.Impl_hacl.sign (Core_models.Ops.Deref.f_deref #(Alloc.Vec.t_Vec u8
+                  Alloc.Alloc.t_Global)
+              #FStar.Tactics.Typeclasses.solve
+              preimage
+            <:
+            t_Slice u8)
+          (Core_models.Convert.f_as_ref #Libcrux_ed25519.Impl_hacl.t_SigningKey
+              #(t_Array u8 (mk_usize 32))
+              #FStar.Tactics.Typeclasses.solve
+              self.f_sk
+            <:
+            t_Array u8 (mk_usize 32))
+        <:
+        Core_models.Result.t_Result (t_Array u8 (mk_usize 64)) Libcrux_ed25519.Impl_hacl.t_Error)
+      "Signing should not fail with valid key"
+  in
+  impl_12__from_bytes #v_D bytes
+
+/// Get the raw bytes of this verification key.
+let impl_VerifyingKey__into_bytes (self: t_VerifyingKey) : t_Array u8 (mk_usize 32) =
+  Libcrux_ed25519.Impl_hacl.impl_VerificationKey__into_bytes self._0
+
+/// Verify `sig` over `msg`. The domain is determined by the type of `sig`.
+/// Returns an error if the signature is invalid.
+let impl_VerifyingKey__verify
+      (#v_D: Type0)
+      (#[FStar.Tactics.Typeclasses.tcresolve ()] i0: t_DomainTag v_D)
+      (self: t_VerifyingKey)
+      (msg: t_Slice u8)
+      (sig: t_Signature v_D)
+    : Core_models.Result.t_Result Prims.unit Anyhow.t_Error =
+  let preimage:Alloc.Vec.t_Vec u8 Alloc.Alloc.t_Global = tagged_preimage #v_D msg in
+  Core_models.Result.impl__map_err #Prims.unit
+    #Libcrux_ed25519.Impl_hacl.t_Error
+    #Anyhow.t_Error
+    (Libcrux_ed25519.Impl_hacl.verify (Core_models.Ops.Deref.f_deref #(Alloc.Vec.t_Vec u8
+                Alloc.Alloc.t_Global)
+            #FStar.Tactics.Typeclasses.solve
+            preimage
+          <:
+          t_Slice u8)
+        (Core_models.Convert.f_as_ref #Libcrux_ed25519.Impl_hacl.t_VerificationKey
+            #(t_Array u8 (mk_usize 32))
+            #FStar.Tactics.Typeclasses.solve
+            self._0
+          <:
+          t_Array u8 (mk_usize 32))
+        sig.f_bytes
+      <:
+      Core_models.Result.t_Result Prims.unit Libcrux_ed25519.Impl_hacl.t_Error)
+    (fun temp_0_ ->
+        let _:Libcrux_ed25519.Impl_hacl.t_Error = temp_0_ in
+        let error:Anyhow.t_Error =
+          Anyhow.__private.format_err (Core_models.Fmt.Rt.impl_1__new_const (mk_usize 1)
+                (let list = ["Signature verification failed"] in
+                  FStar.Pervasives.assert_norm (Prims.eq2 (List.Tot.length list) 1);
+                  Rust_primitives.Hax.array_of_list 1 list)
+              <:
+              Core_models.Fmt.t_Arguments)
+        in
+        Anyhow.__private.must_use error)
